Output.fst
@@ -3,6 +3,18 @@ module Output
 open FStar.String
 open FStar.List.Tot
 
+let rec smaller' #t p ref (l: list t {l << ref /\ for_all p l})
+  : (r: list (x: t {x << ref /\ p x}) { length l == length r })
+  = match l with
+  | [] -> []
+  | hd::tl -> hd::smaller' #t p ref tl
+
+let rec smaller #t ref (l: list t {l << ref})
+  : (r: list (x: t {x << ref}) { length l == length r })
+  = match l with
+  | [] -> []
+  | hd::tl -> hd::smaller #t ref tl
+
 type mrange = int * int * int
 
 type output =
@@ -13,21 +25,21 @@ type output =
   | OSeparatedList: separator:output -> items: list output -> output
   | ONest: list output -> output
   | OEmpty
-
-let rec string_of_output' (tab: string) (o: output)
-  = let map_self tab (l: list output) = map (fun x -> admit (); string_of_output' tab x) (admit (); l) in 
+  
+let rec string_of_output' (tab: string) (o: output): Tot _ (decreases o)
+  = let map_self tab l = map (fun x -> string_of_output' tab x) l in 
     match o with
   | OPair jump left right content -> 
           let nl0 = if jump then "\n" ^ tab else "" in
           let tab = if jump then tab ^ "  " else "" in
           let nl1 = if jump then "\n" ^ tab else "" in
-          left ^ nl0 ^ (String.concat "" (map_self tab content)) ^ nl1 ^ right 
+          left ^ nl0 ^ (String.concat "" (map_self tab (smaller o content))) ^ nl1 ^ right 
   | OQuote content -> "\"" ^ content ^ "\""
   | OIdentitier _ name -> name
   | OKeyword spaced kwd -> let s = if spaced then " " else "" in
                           s ^ kwd ^ s
-  | OSeparatedList sep items -> (String.concat (string_of_output' tab sep) (map_self tab items))
-  | ONest l -> String.concat "" (map_self tab l)
+  | OSeparatedList sep items -> (String.concat (string_of_output' tab sep) (map_self tab (smaller o items)))
+  | ONest l -> String.concat "" (map_self tab (smaller o l))
   | OEmpty -> ""
 
 let string_of_output = string_of_output' ""
